Alternative implementation of chacha20_core with tuples But not proven functionally correct yet

code/chacha20/Hacl.Impl.Chacha20.Core32.fst
@@ -101,6 +101,13 @@ let line st a b d r =
   st.(a) <- sta;
   st.(d) <- std
 
+inline_for_extraction val line_alt: a:uint32 -> b:uint32 -> d:uint32 -> r:rotval U32 -> Tot (uint32 & uint32)
+inline_for_extraction let line_alt sta stb std r =
+  let sta = sta +. stb in
+  let std = std ^. sta in
+  let std = rotate_left std r in
+  (sta, std)
+
 inline_for_extraction
 val quarter_round: st:state -> a:index -> b:index -> c:index -> d:index -> Stack unit
 		  (requires (fun h -> live h st /\ v a <> v d /\ v c <> v b))
@@ -113,11 +120,41 @@ let quarter_round st a b c d =
     line st a b d (size 8);
     line st c d b (size 7)
 
+type quarter_state_alt = uint32 & uint32 & uint32 & uint32
+
+inline_for_extraction val quarter_round_alt: quarter_state_alt -> Tot quarter_state_alt
+inline_for_extraction let quarter_round_alt qs =
+  let (a, b, c, d) = qs in
+  let (a, d) = line_alt a b d (size 16) in
+  let (c, b) = line_alt c d b (size 12) in
+  let (a, d) = line_alt a b d (size 8) in
+  let (c, b) = line_alt c d b (size 7) in
+  (a, b, c, d)
+
+type state_alt = quarter_state_alt & quarter_state_alt & quarter_state_alt & quarter_state_alt
+
+inline_for_extraction val double_round_alt: st: state_alt -> Tot state_alt
+inline_for_extraction let double_round_alt st =
+  let ((s0, s1, s2, s3), (s4, s5, s6, s7), (s8, s9, s10, s11), (s12, s13, s14, s15)) = st in
+  let (s0, s4, s8, s12) = quarter_round_alt (s0, s4, s8, s12) in
+  let (s1, s5, s9, s13) = quarter_round_alt (s1, s5, s9, s13) in
+  let (s2, s6, s10, s14) = quarter_round_alt (s2, s6, s10, s14) in
+  let (s3, s7, s11, s15) = quarter_round_alt (s3, s7, s11, s15) in
+
+  let (s0, s5, s10, s15) = quarter_round_alt (s0, s5, s10, s15) in
+  let (s1, s6, s11, s12) = quarter_round_alt (s1, s6, s11, s12) in
+  let (s2, s7, s8, s13) = quarter_round_alt (s2, s7, s8, s13) in
+  let (s3, s4, s9, s14) = quarter_round_alt (s3, s4, s9, s14) in
+  ((s0, s1, s2, s3), (s4, s5, s6, s7), (s8, s9, s10, s11), (s12, s13, s14, s15))
+
+
 [@ CInline]
 val double_round: st:state -> Stack unit
 		  (requires (fun h -> live h st))
 		  (ensures (fun h0 _ h1 -> modifies (loc st) h0 h1 /\
-		    as_seq h1 st == Spec.double_round (as_seq h0 st)))
+	
+	            as_seq h1 st == Spec.double_round (as_seq h0 st)))
+(*
 [@ CInline]
 let double_round st =
   quarter_round st (size 0) (size 4) (size 8) (size 12);
@@ -129,3 +166,43 @@ let double_round st =
   quarter_round st (size 1) (size 6) (size 11) (size 12);
   quarter_round st (size 2) (size 7) (size 8) (size 13);
   quarter_round st (size 3) (size 4) (size 9) (size 14)
+*)
+
+[@ CInline]
+let double_round st =
+  let s0 = Lib.Buffer.index st (size 0) in
+  let s1 = Lib.Buffer.index st (size 1) in
+  let s2 = Lib.Buffer.index st (size 2) in
+  let s3 = Lib.Buffer.index st (size 3) in
+  let s4 = Lib.Buffer.index st (size 4) in
+  let s5 = Lib.Buffer.index st (size 5) in
+  let s6 = Lib.Buffer.index st (size 6) in
+  let s7 = Lib.Buffer.index st (size 7) in
+  let s8 = Lib.Buffer.index st (size 8) in
+  let s9 = Lib.Buffer.index st (size 9) in
+  let s10 = Lib.Buffer.index st (size 10) in
+  let s11 = Lib.Buffer.index st (size 11) in
+  let s12 = Lib.Buffer.index st (size 12) in
+  let s13 = Lib.Buffer.index st (size 13) in
+  let s14 = Lib.Buffer.index st (size 14) in
+  let s15 = Lib.Buffer.index st (size 15) in
+  let ((s0, s1, s2, s3), (s4, s5, s6, s7), (s8, s9, s10, s11), (s12, s13, s14, s15)) =
+    double_round_alt ((s0, s1, s2, s3), (s4, s5, s6, s7), (s8, s9, s10, s11), (s12, s13, s14, s15))
+  in
+  Lib.Buffer.upd st (size 0) s0;
+  Lib.Buffer.upd st (size 1) s1;
+  Lib.Buffer.upd st (size 2) s2;
+  Lib.Buffer.upd st (size 3) s3;
+  Lib.Buffer.upd st (size 4) s4;
+  Lib.Buffer.upd st (size 5) s5;
+  Lib.Buffer.upd st (size 6) s6;
+  Lib.Buffer.upd st (size 7) s7;
+  Lib.Buffer.upd st (size 8) s8;
+  Lib.Buffer.upd st (size 9) s9;
+  Lib.Buffer.upd st (size 10) s10;
+  Lib.Buffer.upd st (size 11) s11;
+  Lib.Buffer.upd st (size 12) s12;
+  Lib.Buffer.upd st (size 13) s13;
+  Lib.Buffer.upd st (size 14) s14;
+  Lib.Buffer.upd st (size 15) s15;
+  admit()
